Proof of progress for basic linear lambda calculus.
Also, more modules and more things copied over from SfLib.

Syntax.v
@@ -2,13 +2,28 @@ Require Import DbLib.DeBruijn.
 Require Import DbLib.Environments.
 Require Import DbLib.DblibTactics.
 Require Import PartialMap.
-
-Module Syntax.
+Require Import Util.
 
 (* We use natural numbers as De Bruijn indices to denote term and location variables. *)
 Inductive name := Name : nat -> name.
 (* No distinction between location variables and constants. *)
 Inductive loc := Loc : nat -> loc.
+
+Inductive ty : Type :=
+  | TyUnit
+  (*
+  | TyProduct : ty -> ty -> ty
+  *)
+  | TyFun : ty -> ty -> ty
+  (*
+  | TyBang : ty -> ty
+  | TyPtr : loc -> ty
+  | TyCap : loc -> ty -> ty
+  | TyForAll : ty -> ty
+  | TyEx : ty -> ty
+  *)
+  | TyBool
+.
 
 (* Terms, or 'expressions' in L3 parlance. *)
 Inductive term : Type :=
@@ -26,7 +41,8 @@ Inductive term : Type :=
   *)
   (* FIXME: Would be nice to use name type, but prove_*_traverse tactics choke. *)
   | TVar : nat -> term
-  | TAbs : term -> term
+  (* (\0: tau. e *)
+  | TAbs : ty -> term -> term
   | TApp : term -> term -> term
   (*
   (* FIXME: Need a value bound here? *)
@@ -47,28 +63,18 @@ Inductive term : Type :=
   *)
 .
 
-Inductive value : term -> Type :=
+Hint Constructors term.
+
+Inductive value : term -> Prop :=
   | VUnit : value TUnit
-  | VAbs : forall e, value (TAbs e)
+  | VVar : forall x, value (TVar x)
+  | VAbs : forall t e, value (TAbs t e)
   | VTrue : value TTrue
   | VFalse : value TFalse
 .
 
-Inductive ty : Type :=
-  | TyUnit
-  (*
-  | TyProduct : ty -> ty -> ty
-  *)
-  | TyFunc : ty -> ty -> ty
-  (*
-  | TyBang : ty -> ty
-  | TyPtr : loc -> ty
-  | TyCap : loc -> ty -> ty
-  | TyForAll : ty -> ty
-  | TyEx : ty -> ty
-  *)
-  | TyBool
-.
+Hint Constructors value.
+
 
 (* ---------------------- *)
 (* Substitution via DbLib *)
@@ -87,8 +93,8 @@ Fixpoint traverse_term (f : nat -> nat -> term) l t :=
   | TFalse => TFalse
   | TVar x =>
       f l x
-  | TAbs e =>
-      TAbs (traverse_term f (1 + l) e)
+  | TAbs t e =>
+      TAbs t (traverse_term f (1 + l) e)
   | TApp e1 e2 =>
       TApp (traverse_term f l e1) (traverse_term f l e2)
   end.
@@ -147,13 +153,14 @@ Inductive eval_ctxt : term -> term -> Prop :=
       eval_ctxt (TPair E e2) (TPair e1 e2)
   *)
 .
+(* ^ NOT USED *)
 
 (* (sigma, e) -> (sigma', e') *)
 Inductive step : store -> term -> store -> term -> Prop :=
-  | StepAppAbs : forall s e e' v,
+  | StepAppAbs : forall s e e' v t,
       value v ->
       subst v 0 e = e' ->
-      step s (TApp (TAbs e) v) s e'
+      step s (TApp (TAbs t e) v) s e'
   | StepApp1 : forall s s' e1 e1' e2,
       step s e1 s' e1' ->
       step s (TApp e1 e2) s' (TApp e1' e2)
@@ -163,12 +170,133 @@ Inductive step : store -> term -> store -> term -> Prop :=
       step s (TApp v1 e2) s' (TApp v1 e2')
 .
 
+Hint Constructors step.
+
+(* Typing judgements *)
+Definition loc_ctxt := PartialMap.partial_map unit.
+Definition ty_ctxt := PartialMap.partial_map ty.
+
+
+Reserved Notation "LC ';' VC '|-' t '~:' T" (at level 40).
+
+(* TODO: Work out context splitting. Probably doesn't work well with partial maps... *)
+
+(* Adapted from de Vries *)
+Inductive context_split : ty_ctxt -> ty_ctxt -> ty_ctxt -> Prop :=
+  | split_empty : context_split empty empty empty
+  (* Might need to check that x not in E *)
+  | split_left : forall E E1 E2 x t,
+      E x = None ->
+      context_split E E1 E2 ->
+      context_split (extend E x t) (extend E1 x t) E2
+  | split_right : forall E E1 E2 x t,
+      E x = None ->
+      context_split E E1 E2 ->
+      context_split (extend E x t) E1 (extend E2 x t)
+.
+
+Hint Constructors context_split.
+
+Lemma empty_context : forall E1 E2,
+  context_split empty E1 E2 -> E1 = empty /\ E2 = empty.
+Proof.
+  intros E1 E2 H.
+  inversion H.
+  (* Split empty *)
+  auto.
+  (* Split left *)
+  unfold not in H0. apply extend_neq_empty in H0. inversion H0.
+  admit.
+Qed.
+
+Lemma split_complete : forall E E1 E2 x t,
+  context_split E E1 E2 ->
+  E x = Some t ->
+  (E1 x = Some t) \/ (E2 x = Some t).
+Proof.
+  intros.
+  induction H.
+  (* Case split_empty *)
+  inversion H0.
+  (* Case split_left *)
+  destruct (eq_nat_dec x x0).
+    (* Equal *)
+    subst x0.
+    left.
+    rewrite extend_eq in H0.
+    inversion H0. subst t0.
+    apply extend_eq.
+    (* Not equal *)
+    rewrite extend_neq in H0.
+    rewrite extend_neq; auto. auto.
+  (* Case split_right *)
+  destruct (eq_nat_dec x x0).
+    subst x0.
+    right.
+    rewrite extend_eq in H0.
+    inversion H0. subst t0.
+    apply extend_eq.
+    (* Not equal *)
+    rewrite extend_neq in H0.
+    rewrite extend_neq; auto. auto.
+Qed.
+
+Inductive has_type : loc_ctxt -> ty_ctxt -> term -> ty -> Prop :=
+  | HasTyUnit : forall LC VC,
+      LC; VC |- TUnit ~: TyUnit
+  | HasTyTrue : forall LC VC,
+      LC; VC |- TTrue ~: TyBool
+  | HasTyFalse : forall LC VC,
+      LC; VC |- TFalse ~: TyBool
+  | HasTyVar : forall LC VC x t,
+      VC x = Some t ->
+      LC; VC |- TVar x ~: t
+  (* FIXME: Shifting...? *)
+  | HasTyAbs : forall LC VC e t1 t2,
+      LC; (extend VC 0 t1) |- e ~: t2 ->
+      LC; VC |- TAbs t1 e ~: TyFun t1 t2
+  | HasTyApp : forall LC E E1 E2 e1 e2 t1 t2,
+      context_split E E1 E2 ->
+      LC; E1 |- e1 ~: TyFun t1 t2 ->
+      LC; E2 |- e2 ~: t1 ->
+      LC; E  |- TApp e1 e2 ~: t2
+
+where "LC ';' VC '|-' t '~:' T" := (has_type LC VC t T).
+
+Hint Constructors has_type.
 
 
 
-
-
-
-
-
-End Syntax.
+(* Time to prove progress *)
+Theorem progress : forall L E e s t,
+  (* Hacks to prevent empty from disappearing during induction *)
+  L = empty ->
+  E = empty ->
+  L; E |- e ~: t ->
+  (exists s' e', step s e s' e') \/ value e.
+Proof with eauto.
+  intros L E e s t Ln En H.
+  induction H; auto.
+  (* Application *)
+  (* First, reasoning about the context splitting. We want E1 = E2 = empty. *)
+  subst E. apply empty_context in H. destruct H as [E1empty E2empty].
+  destruct IHhas_type1...
+  (* e1 steps *)
+  Case "e1 steps".
+    (* Proof by StepApp1 (invert stepping of e1) *)
+    inversion H. inversion H2... (* FIXME: tactic here *)
+  Case "e1 is a value".
+    destruct IHhas_type2 as [IH1 | IH2]...
+    SCase "e2 steps".
+      inversion IH1... inversion H2... (* Same tactic needed here *)
+    SCase "e2 is a value".
+      (* Here we use beta reduction, by first showing that e1 must be a lambda expression *)
+      left.
+      destruct e1; try (solve by inversion).
+      (* Var case is impossible *)
+      inversion H0; subst.
+      solve by inversion.
+      (* Beta reduction! *)
+      exists s.
+      exists (subst e2 0 e1)...
+Qed.
