PartialMap.v
@@ -1,37 +1,10 @@
 (* PartialMap implementation adapted from Ben Pierce's Software Foundations *)
-Module PartialMap.
-
-(* Decision procedure for nat equality and some theorems about it. *)
-Theorem eq_nat_dec : forall (n m : nat), {n = m} + {n <> m}.
-Proof.
-  decide equality.
-Defined.
-
-Theorem eq_id : forall (T: Type) n (p q: T), (if eq_nat_dec n n then p else q) = p.
-Proof.
-  intros T n p q.
-  destruct (eq_nat_dec n n).
-    reflexivity.
-    assert False as contra; auto. inversion contra.
-Qed.
-
-Theorem neq_id : forall (T: Type) n1 n2 (p q: T),
-  n1 <> n2 ->
-  (if eq_nat_dec n1 n2 then p else q) = q.
-Proof.
-  intros T n1 n2 p q neq.
-  destruct (eq_nat_dec n1 n2).
-    assert False as contra; auto. inversion contra.
-    reflexivity.
-Qed.
+Require Import Util.
+Require Import Coq.Logic.FunctionalExtensionality.
 
 Definition partial_map (A : Type) := nat -> option A.
 
 Definition empty {A:Type} : partial_map A := (fun _ => None).
-
-(** Informally, we'll write [Gamma, x:T] for "extend the partial
-    function [Gamma] to also map [x] to [T]."  Formally, we use the
-    function [extend] to add a binding to a partial map. *)
 
 Definition extend {A:Type} (Gamma : partial_map A) (x : nat) (T : A) :=
   fun x' => if eq_nat_dec x x' then Some T else Gamma x'.
@@ -49,4 +22,12 @@ Proof.
   intros. unfold extend. rewrite neq_id; auto.
 Qed.
 
-End PartialMap.
+Lemma extend_neq_empty : forall A (ctxt : partial_map A) x T,
+  extend ctxt x T <> empty.
+Proof.
+  unfold not.
+  intros.
+  admit.
+Qed.
+
+
