Util.v
@@ -1,0 +1,67 @@
+(* Decision procedure for nat equality, and some theorems about it. *)
+Theorem eq_nat_dec : forall (n m : nat), {n = m} + {n <> m}.
+Proof.
+  decide equality.
+Defined.
+
+Theorem eq_id : forall (T: Type) n (p q: T), (if eq_nat_dec n n then p else q) = p.
+Proof.
+  intros T n p q.
+  destruct (eq_nat_dec n n).
+    reflexivity.
+    assert False as contra; auto. inversion contra.
+Qed.
+
+Theorem neq_id : forall (T: Type) n1 n2 (p q: T),
+  n1 <> n2 ->
+  (if eq_nat_dec n1 n2 then p else q) = q.
+Proof.
+  intros T n1 n2 p q neq.
+  destruct (eq_nat_dec n1 n2).
+    assert False as contra; auto. inversion contra.
+    reflexivity.
+Qed.
+
+(* Solve by inversion tactic nicked from SfLib *)
+Tactic Notation "solve_by_inversion_step" tactic(t) :=
+  match goal with
+  | H : _ |- _ => solve [ inversion H; subst; t ]
+  end
+  || fail "because the goal is not solvable by inversion.".
+
+Tactic Notation "solve" "by" "inversion" "1" :=
+  solve_by_inversion_step idtac.
+Tactic Notation "solve" "by" "inversion" "2" :=
+  solve_by_inversion_step (solve by inversion 1).
+Tactic Notation "solve" "by" "inversion" "3" :=
+  solve_by_inversion_step (solve by inversion 2).
+Tactic Notation "solve" "by" "inversion" :=
+  solve by inversion 1.
+
+(* Case markers also nicked from SF *)
+Require String. Open Scope string_scope.
+
+Ltac move_to_top x :=
+  match reverse goal with
+  | H : _ |- _ => try move x after H
+  end.
+
+Tactic Notation "assert_eq" ident(x) constr(v) :=
+  let H := fresh in
+  assert (x = v) as H by reflexivity;
+  clear H.
+
+Tactic Notation "Case_aux" ident(x) constr(name) :=
+  first [
+    set (x := name); move_to_top x
+  | assert_eq x name; move_to_top x
+  | fail 1 "because we are working on a different case" ].
+
+Tactic Notation "Case" constr(name) := Case_aux Case name.
+Tactic Notation "SCase" constr(name) := Case_aux SCase name.
+Tactic Notation "SSCase" constr(name) := Case_aux SSCase name.
+Tactic Notation "SSSCase" constr(name) := Case_aux SSSCase name.
+Tactic Notation "SSSSCase" constr(name) := Case_aux SSSSCase name.
+Tactic Notation "SSSSSCase" constr(name) := Case_aux SSSSSCase name.
+Tactic Notation "SSSSSSCase" constr(name) := Case_aux SSSSSSCase name.
+Tactic Notation "SSSSSSSCase" constr(name) := Case_aux SSSSSSSCase name.
